up to prop2.3

src/basic.lean
@@ -1,13 +1,33 @@
 import tactic
 
+-- Definition 2.1
 structure filter (X : Type*) :=
 (sets                     : set (set X))
 (upward_closure {F₁ F₂}   : F₁ ∈ sets → F₁ ⊆ F₂ → F₂ ∈ sets)
 (inter_sets {F₁ F₂}       : F₁ ∈ sets → F₂ ∈ sets → F₁ ∩ F₂ ∈ sets)
 
-instance {X : Type*}: has_mem (set X) (filter X) := ⟨λ U F, U ∈ F.sets⟩
+instance {X : Type*} : has_mem (set X) (filter X) := ⟨λ U F, U ∈ F.sets⟩
 
-namespace filter
+variables {X : Type*} {f g : filter X} {s : set X}
 
+@[simp] lemma filter.mem_sets : s ∈ f.sets ↔ s ∈ f := iff.rfl
 
-end filter
+-- Definition 2.2
+structure filter_basis (X : Type*) :=
+(sets                   : set (set X))
+(inter_sets {x y}       : x ∈ sets → y ∈ sets → ∃ z ∈ sets, z ⊆ x ∩ y)
+--(nonempty               : sets.nonempty)
+
+instance {X : Type*} : has_mem (set X) (filter_basis X) := sorry
+
+protected def filter_basis.filter (B : filter_basis X) : filter X :=
+{ sets := {s | ∃ t ∈ B, t ⊆ s},
+  upward_closure := sorry,
+  inter_sets := sorry, }
+
+-- Prop 2.3
+def filter.as_basis (f : filter X) : filter_basis X :=
+⟨f.sets, sorry⟩
+
+-- Prop 2.4
+
